extend_vals in terms of destruct_member

src/LLG.v
@@ -77,120 +77,15 @@ Section LLG.
     | TArray _ => ListIsArray _ nil
     end.
 
-(*
-  Definition fill_in_type(x: var)(t: nat)(l: list var)(types: member (remove eq_var_dec x l) -> nat):
-    (member l -> nat) :=
-    fun m => match (eq_var_dec (member_get m) x) with
-      | left _ => t
-      | right NEq => types (member_remove eq_var_dec x l m NEq)
-      end.
-
-  Definition fill_in_val(x: var)(t: nat)(v: interp_type t)(l: list var)
-    (R: member (remove eq_var_dec x l) -> nat)
-    (vals: forall m : member (remove eq_var_dec x l), interp_type (R m)):
-    (forall m: member l, interp_type (fill_in_type x t l R m)).
-    intro m.
-    unfold fill_in_type.
-    destruct (eq_var_dec (member_get m) x).
-    + exact v.
-    + apply (vals (member_remove eq_var_dec x l m n)).
-  Defined.
-*)
-
-(*  Definition fill_in_val{tx: nat}(x: var)(v: interp_type tx)(l: list var)
-    (R: member (remove eq_var_dec x l) -> V)
-    (vals: forall (m: member (remove eq_var_dec x l)), R m):
-    (forall (m: member l), R m). :=
-    fun m => match (eq_var_dec (member_get m) x) with
-      | left _ => t
-      | right NEq => types (member_remove eq_var_dec x l m NEq)
-      end.
-*)
-(*
-  Definition fill_in_val{V: Type}(x: var)(v: V)(l: list var)(R: member (remove eq_var_dec x l) -> V)
-    (vals: forall (m: member (remove eq_var_dec x l)), R m):
-    (forall (m: member l), R m). :=
-    fun m => match (eq_var_dec (member_get m) x) with
-      | left _ => t
-      | right NEq => types (member_remove eq_var_dec x l m NEq)
-      end.
-*)
-
-(*
-  Definition update_vals(l: list var)(types: member l -> Type)(i: member l)(v: types i)
-    (vals: forall m : member l, types m):
-           forall m : member l, types m.
-    intro m.
-    (* destruct (eq_var_dec (member_get i) (member_get m)). bad because member_get not injective *)
-    destruct (eq_member_dec _ i m).
-    - rewrite <- e. exact v.
-    - exact (vals m).
-  Defined.
-*)
-
-Require Import lib.LibTactics.
-
-
-  Definition interp_expr{l G t}: 
-    forall (e: expr l G t)(vals: forall x: member l, interp_type (G x)), interp_type t.
-    refine (fix rec (e: expr l G t)(vals: forall x: member l, interp_type (G x))
-               {struct e}: interp_type t :=
-      match e with
-      | ELit v => _
-      | EVar m => _
-      | EOp e1 op e2 => _
-      | ELet x e1 e2 => _
-      end).
-      - exact v.
-      - Fail exact (vals m).
-  Abort.
-
-  Definition interp_expr{l G t}: 
-    forall (e: expr l G t)(vals: forall x: member l, interp_type (G x)), interp_type t.
-    refine (fix rec (e: expr l G t) :=
-      match e in (expr l G t) return ((forall x: member l, interp_type (G x)) -> interp_type t) with
-      | ELit v => fun vals => v
-      | EVar m => fun vals => vals m
-      | EOp e1 op e2 => fun vals => _
-      | ELet x e1 e2 => _
-      end).
-      - Fail exact (eval_binop_nat op (rec e1 vals) (rec e2 vals)).
-  Abort.
-
   Definition extend_vals:
     forall {l} (G: member l -> type)(vals: forall m: member l, interp_type (G m))
     (x: var)(t: type)(v: interp_type t),
     forall m: member (x :: l), interp_type (extend G x t m).
-    Admitted. (*
-  refine (fun l G vals x t v m => 
-    match m with
-    | member_here _ _ => fun l G vals m => _
-    | member_there _ _ _ => fun l G vals m => _
-    end l G vals).
-
-  Definition extend_vals:
-    forall l (G: member l -> type)(vals: forall m: member l, interp_type (G m))
-    (x: var)(t: type)(v: interp_type t),
-    forall m: member (x :: l) -> interp_type (extend G x t m).
-  refine (fun l G vals x t v m => 
-    match m with
-    | member_here _ _ => fun l G vals m => _
-    | member_there _ _ _ => fun l G vals m => _
-    end l G vals).
-    - unfold extend. 
-
-  Definition extend_vals{l}(G: member l -> type)(vals: forall m: member l, interp_type (G m))
-    (x: var)(t: type)(v: interp_type t):
-    forall m: member (x :: l) -> interp_type (extend G x t m) :=
-    refine (
-    intro m. destruct m.
-    
-     :=
-    fun m => match m with (* (fancy return clause inferred) *)
-    | member_here _ _ => fun _ => t
-    | member_there _ _ m' => fun G => G m'
-    end G.
-*)
+    intros.
+    apply (destruct_member m).
+    - intro E. subst m. simpl. exact v.
+    - intros m' E. subst m. simpl. exact (vals m').
+  Defined.
 
   Definition interp_expr:
     forall {l G t}(e: expr l G t)(vals: forall x: member l, interp_type (G x)), interp_type t :=
@@ -205,110 +100,28 @@ Require Import lib.LibTactics.
           rec _ _ _ e2 vals'
       end.
 
-(*
-  Fixpoint interp_expr{n: nat}{l: list var}
-    (e: expr l n) (types: member l -> nat)
-    {struct e}:
-      option ((forall x: member l, interp_type (types x)) -> interp_type n).
-    destruct e eqn: E.
-    - simpl. apply Some. intro vals. exact v.
-    - destruct (Nat.eq_dec n (types (member_here x []))).
-      + subst n. apply Some.
-        intro vals. set (v := vals (member_here x nil)).
-        apply v.
-      + exact None. (* error: types list doesn't match *)
-    - set (o1 := interp_expr _ l1 e0_1 (fun m => types (member_app_r l1 l2 m))).
-      simpl in o1.
-      destruct o1 as [f1|].
-      + set (o2 := interp_expr _ l2 e0_2 (fun m => types (member_app_l l1 l2 m))).
-        simpl in o2.
-        destruct o2 as [f2|].
-        * apply Some. intro vals.
-          specialize (f1 (fun m => vals (member_app_r l1 l2 m))).
-          specialize (f2 (fun m => vals (member_app_l l1 l2 m))).
-          exact (eval_binop_nat op f1 f2).
-        * exact None.
-      + exact None.
-    - set (o1 := interp_expr n1 l1 e0_1
-        (fun (m: member l1) => types (member_app_r l1 (remove eq_var_dec x l2) m))).
-      destruct o1 as [f1|].
-      + set (types' := (fun m => types (member_app_l l1 (remove eq_var_dec x l2) m))).
-        set (types'' := fill_in_type x n1 l2 types').
-        set (o2 := interp_expr n2 l2 e0_2 types'').
-        destruct o2 as [f2|].
-        * apply Some. intro vals.
-          specialize (f1 (fun (m: member l1) => vals  (member_app_r l1 (remove eq_var_dec x l2) m))).
-          set (vals' := (fun m => vals (member_app_l l1 (remove eq_var_dec x l2) m))).
-          replace (forall m : member (remove eq_var_dec x l2),
-                   interp_type (types (member_app_l l1 (remove eq_var_dec x l2) m)))
-             with (forall m : member (remove eq_var_dec x l2),
-                   interp_type (types' m)) in vals'
-             by (subst types'; reflexivity).
-          subst types''.
-          set (vals'' := fill_in_val x n1 f1 l2 types' vals').
-          exact (f2 vals'').
-        * exact None.
-      + exact None.
-    - set (o := interp_expr 0 l e0 types).
-      simpl in o.
-      destruct o as [f|].
-      + apply Some. intro vals.
-        specialize (f vals).
-        exact (@newArray _ _ (interp_type_IsArray n) f).
-      + exact None.
-    - set (o1 := interp_expr _ l1 e0_1 (fun m => types (member_app_r l1 l2 m))).
-      simpl in o1.
-      destruct o1 as [f1|].
-      + set (o2 := interp_expr _ l2 e0_2 (fun m => types (member_app_l l1 l2 m))).
-        simpl in o2.
-        destruct o2 as [f2|].
-        * apply Some. intro vals.
-          specialize (f1 (fun m => vals (member_app_r l1 l2 m))).
-          specialize (f2 (fun m => vals (member_app_l l1 l2 m))).
-          exact (@get _ _ (interp_type_IsArray n) f1 f2).
-        * exact None.
-      + exact None.
-    - set (o1 := interp_expr _ l1 e0_1
-        (fun m => types (member_app_13 l1 l2 l3 m))).
-      simpl in o1.
-      destruct o1 as [f1|].
-      + set (o2 := interp_expr _ l2 e0_2 (fun m => types (member_app_23 l1 l2 l3 m))).
-        simpl in o2.
-        destruct o2 as [f2|].
-        * set (o3 := interp_expr _ l3 e0_3 (fun m => types (member_app_33 l1 l2 l3 m))).
-          destruct o3 as [f3|].
-          { apply Some. intro vals.
-            specialize (f1 (fun m => vals  (member_app_13 l1 l2 l3 m))).
-            specialize (f2 (fun m => vals  (member_app_23 l1 l2 l3 m))).
-            specialize (f3 (fun m => vals  (member_app_33 l1 l2 l3 m))).
-            exact (@update _ _ (interp_type_IsArray n) f1 f2 f3). }
-          { exact None. }
-        * exact None.
-      + exact None.
-  Defined.
-*)
 End LLG.
-(*
+
 Definition test1(v1 v2: nat): nat := let x1 := v1 in let x2 := v2 in x1.
 
 Definition myvar := nat.
 Definition var_x1: myvar := 1.
 Definition var_x2: myvar := 2.
 
-Definition test1a(v1 v2: nat): expr (@nil myvar) 0 :=
-  ELet var_x1 (ELit v1) (ELet var_x2 (ELit v2) (EVar 0 var_x1)).
-
-Definition empty_types: member (@nil myvar) -> nat. intro. inversion H. Defined.
+Definition empty_types: member (@nil myvar) -> type. intro. inversion H. Defined.
 Definition empty_vals: forall m : member (@nil myvar), interp_type (empty_types m).
   intro. inversion m. Defined.
 
-Definition interp_expr'{n: nat}(e: expr (@nil myvar) n): option (interp_type n) :=
-  match interp_expr e empty_types with
-  | Some f => Some (f empty_vals)
-  | None => None
-  end.
+Definition x1_in_x2x1: member [var_x2; var_x1]. apply member_there. apply member_here. Defined.
+Definition x2_in_x2x1: member [var_x2; var_x1]. apply member_here. Defined.
 
-Goal forall v1 v2, Some (test1 v1 v2) = interp_expr' (test1a v1 v2).
+Definition test1a(v1 v2: nat): expr (@nil myvar) empty_types TNat :=
+  ELet var_x1 (ELit v1) (ELet var_x2 (ELit v2) (EVar x1_in_x2x1)).
+
+Definition interp_expr'{t}(e: expr (@nil myvar) empty_types t): interp_type t :=
+  interp_expr e empty_vals.
+
+Goal forall v1 v2, test1 v1 v2 = interp_expr' (test1a v1 v2).
   intros. reflexivity.
 Qed.
 
@@ -320,6 +133,7 @@ Definition test2(i v: nat): nat :=
   let x2 := update x1 i v in
   get x2 i.
 
+(*
 Definition test2a(i v: nat): expr (@nil myvar) 0 :=
   ELet var_x1 (ENewArray 0 (ELit 3))
   (ELet var_x2 (EUpdate (EVar 1 var_x1) (ELit i) (ELit v))
